PivotBetree/PivotBetreeSpec.i.dfy
@@ -7,7 +7,7 @@ include "../lib/Base/Option.s.dfy"
 include "../lib/Base/Message.i.dfy"
 include "../Betree/BetreeSpec.i.dfy"
 include "../Betree/Betree.i.dfy"
-include "../lib/Buckets/PivotsLib.i.dfy"
+include "../lib/Buckets/BoundedPivotsLib.i.dfy"
 include "../lib/Buckets/BucketsLib.i.dfy"
 include "../PivotBetree/Bounds.i.dfy"
 include "../lib/Buckets/BucketWeights.i.dfy"
@@ -25,13 +25,11 @@ module PivotBetreeGraph refines Graph {
   import opened ValueMessage
   import opened KeyType
   import opened BucketsLib
+  import opened BoundedPivotsLib
 
   import Keyspace = Lexicographic_Byte_Order
+  import KeyspaceImpl = Lexicographic_Byte_Order_Impl
 
-  //type Reference = BG.Reference
-  //function Root() : Reference { BG.Root() }
-
-  type PivotTable = seq<Key>
   datatype Node = Node(
       pivotTable: PivotTable,
       children: Option<seq<Reference>>,
@@ -58,12 +56,12 @@ module PivotBetreeSpec {
   import opened Maps
   import opened Options
   import opened Bounds
-  import opened PivotsLib
   import opened BucketsLib
   import opened BucketWeights
   import UI
   import opened KeyType
   import opened ValueMessage
+  import opened bpl = BoundedPivotsLib
 
   export Spec provides BetreeStep, ValidBetreeStep, BetreeStepReads, BetreeStepOps, BetreeStepUI, G, WFNode, InvNode
   export Internal reveals *
@@ -97,6 +95,7 @@ module PivotBetreeSpec {
 
   function AddMessageToNode(node: Node, key: Key, msg: Message) : Node
   requires WFNode(node)
+  requires BoundedKey(node.pivotTable, key)
   {
     var newnode := node.(
       buckets := BucketListInsert(node.buckets, node.pivotTable, key, msg)
@@ -144,14 +143,22 @@ module PivotBetreeSpec {
 
   predicate LookupVisitsWellMarshalledBuckets(lookup: Lookup, key: Key)
   requires LookupVisitsWFNodes(lookup)
+  requires LookupBoundedKey(key, lookup)
   {
     forall i :: 0 <= i < |lookup| ==> BucketWellMarshalled(lookup[i].node.buckets[Route(lookup[i].node.pivotTable, key)])
+  }
+
+  predicate LookupBoundedKey(key: Key, lookup: Lookup)
+  requires LookupVisitsWFNodes(lookup)
+  {
+    && (forall idx :: ValidLayerIndex(lookup, idx) ==> BoundedKey(lookup[idx].node.pivotTable, key))
   }
 
   predicate LookupFollowsChildRefAtLayer(key: Key, lookup: Lookup, idx: int)
   requires ValidLayerIndex(lookup, idx)
   requires idx < |lookup| - 1;
   requires WFNode(lookup[idx].node)
+  requires BoundedKey(lookup[idx].node.pivotTable, key)
   {
     && lookup[idx].node.children.Some?
     && lookup[idx].node.children.value[Route(lookup[idx].node.pivotTable, key)] == lookup[idx+1].ref
@@ -159,18 +166,21 @@ module PivotBetreeSpec {
 
   predicate LookupFollowsChildRefs(key: Key, lookup: Lookup)
   requires LookupVisitsWFNodes(lookup)
+  requires LookupBoundedKey(key, lookup)
   {
     && (forall idx :: ValidLayerIndex(lookup, idx) && idx < |lookup| - 1 ==> LookupFollowsChildRefAtLayer(key, lookup, idx))
   }
 
   function NodeLookup(node: Node, key: Key) : Message
   requires WFBucketList(node.buckets, node.pivotTable)
+  requires BoundedKey(node.pivotTable, key)
   {
     BucketListGet(node.buckets, node.pivotTable, key)
   }
 
   function InterpretLookup(lookup: Lookup, key: Key) : Message
   requires LookupVisitsWFNodes(lookup)
+  requires LookupBoundedKey(key, lookup)
   {
     if |lookup| == 0 then
       Update(NopDelta())
@@ -181,6 +191,7 @@ module PivotBetreeSpec {
   function InterpretLookupAccountingForLeaf(lookup: Lookup, key: Key) : Message
   requires |lookup| > 0
   requires LookupVisitsWFNodes(lookup)
+  requires LookupBoundedKey(key, lookup)
   {
     if Last(lookup).node.children.Some? then
       InterpretLookup(lookup, key)
@@ -193,6 +204,7 @@ module PivotBetreeSpec {
     && |lookup| > 0
     && lookup[0].ref == Root()
     && LookupVisitsWFNodes(lookup)
+    && LookupBoundedKey(key, lookup)
     && LookupFollowsChildRefs(key, lookup)
   }
 
@@ -222,10 +234,11 @@ module PivotBetreeSpec {
 
   function LookupUpperBoundAtLayer(layer: Layer, key: Key) : Option<Key>
   requires WFNode(layer.node)
+  requires BoundedKey(layer.node.pivotTable, key)
   {
     var r := Route(layer.node.pivotTable, key);
-    if r < |layer.node.pivotTable|
-    then Some(layer.node.pivotTable[r])
+    if layer.node.pivotTable[r+1].Element? 
+    then Some(GetKey(layer.node.pivotTable, r+1))
     else None
   }
 
@@ -233,7 +246,7 @@ module PivotBetreeSpec {
   {
     match k1 {
       case Some(key1) => match k2 {
-        case Some(key2) => if Keyspace.lt(k1.value, k2.value) then Some(k1.value) else Some(k2.value)
+        case Some(key2) => if G.Keyspace.lt(k1.value, k2.value) then Some(k1.value) else Some(k2.value)
         case None => k1
       }
       case None => k2
@@ -242,6 +255,7 @@ module PivotBetreeSpec {
 
   function {:opaque} LookupUpperBound(lookup: Lookup, key: Key) : Option<Key>
   requires LookupVisitsWFNodes(lookup)
+  requires LookupBoundedKey(key, lookup)
   {
     if lookup == []
     then None
@@ -262,12 +276,12 @@ module PivotBetreeSpec {
     && WFLookupForKey(sq.lookup, startKey)
 
     && var lookupUpperBound := LookupUpperBound(sq.lookup, startKey);
-
     && Last(sq.lookup).node.children.None?
 
     && |sq.lookup| == |sq.buckets|
     && (forall i | 0 <= i < |sq.lookup| :: sq.buckets[i] == sq.lookup[i].node.buckets[Route(sq.lookup[i].node.pivotTable, startKey)])
 
+    // what if sq.end is positive infinity?
     && (BucketListWellMarshalled(sq.buckets) ==> (
       && MS.NonEmptyRange(sq.start, sq.end)
       && (lookupUpperBound.Some? ==> !MS.UpperBound(lookupUpperBound.value, sq.end))
@@ -291,6 +305,7 @@ module PivotBetreeSpec {
 
   predicate ValidInsertion(ins: MessageInsertion) {
     && WFNode(ins.oldroot)
+    && BoundedKey(ins.oldroot.pivotTable, ins.key)
     && WeightBucketList(ins.oldroot.buckets) + WeightKey(ins.key) + WeightMessage(ins.msg)
         <= MaxTotalBucketWeight()
   }
@@ -309,8 +324,17 @@ module PivotBetreeSpec {
     [writeop]
   }
 
-  //// Flush
+  function {:opaque} NodeInsertKeyValue(node: Node, key: Key, msg: Message) : Node
+  requires WFNode(node)
+  requires BoundedKey(node.pivotTable, key)
+  {
+    var r := Route(node.pivotTable, key);
+    var bucket := node.buckets[r];
+    var newBucket := BucketInsert(bucket, key, msg);
+    node.(buckets := node.buckets[r := newBucket])
+  }
 
+  //// Flush
   datatype NodeFlush = NodeFlush(
     parentref: Reference,
     parent: Node,
@@ -333,6 +357,7 @@ module PivotBetreeSpec {
     && f.parent.children.value[f.slotIndex] == f.childref
     && WFBucketList(f.newChildBuckets, f.child.pivotTable)
     && WFBucket(f.newParentBucket)
+    && (forall key | key in f.keys :: BoundedKey(f.child.pivotTable, key))
     && WeightBucketList(f.newChildBuckets) <= MaxTotalBucketWeight()
     && WeightBucket(f.newParentBucket) <= WeightBucket(f.parent.buckets[f.slotIndex])
     && (BucketListWellMarshalled(f.child.buckets)
@@ -375,7 +400,8 @@ module PivotBetreeSpec {
 
   predicate ValidGrow(growth: RootGrowth)
   {
-    WFNode(growth.oldroot)
+    && WFNode(growth.oldroot)
+    && ContainsAllKeys(growth.oldroot.pivotTable)
   }
 
   function GrowReads(growth: RootGrowth) : seq<ReadOp>
@@ -387,7 +413,7 @@ module PivotBetreeSpec {
   function GrowOps(growth: RootGrowth) : seq<Op>
   requires ValidGrow(growth)
   {
-    var newroot := Node([], Some([growth.newchildref]), [B(map[])]);
+    var newroot := Node(InitPivotTable(), Some([growth.newchildref]), [B(map[])]);
     var allocop := G.AllocOp(growth.newchildref, growth.oldroot);
     var writeop := G.WriteOp(Root(), newroot);
     [allocop, writeop]
@@ -413,129 +439,123 @@ module PivotBetreeSpec {
 
   //// Useful functions and lemmas for Split, Merge (other redirects)
 
+  // theses things needs additional proof to prove boundedness 
   function {:opaque} CutoffNodeAndKeepLeft(node: Node, pivot: Key) : (node': Node)
   requires WFNode(node)
+  requires ValidLeftCutOffKey(node.pivotTable, pivot)
   ensures node.children.Some? <==> node'.children.Some?
   ensures WFNode(node')
-  ensures |node'.pivotTable| > 0 ==> Keyspace.lt(Last(node'.pivotTable), pivot)
-  ensures forall key | key in Last(node'.buckets).b :: Keyspace.lt(key, pivot)
+  ensures node'.pivotTable[0] == node.pivotTable[0]
+  ensures Last(node'.pivotTable) == KeyToElement(pivot)
+  ensures forall key | key in Last(node'.buckets).b :: Lexicographic_Byte_Order.lt(key, pivot)
   ensures G.Successors(node') <= G.Successors(node)
   ensures WeightBucketList(node'.buckets) <= WeightBucketList(node.buckets)
   ensures |node'.buckets| <= |node.buckets|
   {
     reveal_SplitBucketLeft();
     var cLeft := CutoffForLeft(node.pivotTable, pivot);
-    var leftPivots := node.pivotTable[.. cLeft];
-    var leftChildren := if node.children.Some? then Some(node.children.value[.. cLeft + 1]) else None;
+    var bplleftPivots := SplitLeft(node.pivotTable, pivot);
+
+    reveal_CutoffForLeft();
+  
+    var leftChildren := if node.children.Some? then Some(node.children.value[.. cLeft+1]) else None;
     var leftBuckets := SplitBucketListLeft(node.buckets, node.pivotTable, cLeft, pivot);
 
     WFSplitBucketListLeft(node.buckets, node.pivotTable, cLeft, pivot);
     WeightSplitBucketListLeft(node.buckets, node.pivotTable, cLeft, pivot);
-
-    Node(leftPivots, leftChildren, leftBuckets)
+    Node(bplleftPivots, leftChildren, leftBuckets)
   }
 
   function {:opaque} CutoffNodeAndKeepRight(node: Node, pivot: Key) : (node': Node)
   requires WFNode(node)
+  requires BoundedKey(node.pivotTable, pivot)
   ensures node.children.Some? <==> node'.children.Some?
   ensures WFNode(node')
-  ensures |node'.pivotTable| > 0 ==> Keyspace.lt(pivot, node'.pivotTable[0])
-  ensures forall key | key in node'.buckets[0].b :: Keyspace.lte(pivot, key)
+  ensures pivot == node'.pivotTable[0].e
+  ensures forall key | key in node'.buckets[0].b :: G.Keyspace.lte(pivot, key)
   ensures G.Successors(node') <= G.Successors(node)
   ensures WeightBucketList(node'.buckets) <= WeightBucketList(node.buckets)
   ensures |node'.buckets| <= |node.buckets|
   {
     reveal_SplitBucketRight();
     var cRight := CutoffForRight(node.pivotTable, pivot);
-    var rightPivots := node.pivotTable[cRight ..];
+    var bplrightPivots := SplitRight(node.pivotTable, pivot);
+
     var rightChildren := if node.children.Some? then Some(node.children.value[cRight ..]) else None;
     var rightBuckets := SplitBucketListRight(node.buckets, node.pivotTable, cRight, pivot);
 
     WFSplitBucketListRight(node.buckets, node.pivotTable, cRight, pivot);
     WeightSplitBucketListRight(node.buckets, node.pivotTable, cRight, pivot);
 
-    Node(rightPivots, rightChildren, rightBuckets)
+    Node(bplrightPivots, rightChildren, rightBuckets)
   }
 
-  lemma CutoffNodeCorrect(node: Node, node1: Node, node2: Node, lpivot: Key, rpivot: Key)
+  predicate ValidSplitKey(node: Node, lpivot: Key, rpivot: Option<Key>)
   requires WFNode(node)
-  requires node1 == CutoffNodeAndKeepLeft(node, rpivot);
-  requires node2 == CutoffNodeAndKeepRight(node1, lpivot);
-  ensures |node2.pivotTable| > 0 ==> Keyspace.lt(lpivot, node2.pivotTable[0])
-  ensures |node2.pivotTable| > 0 ==> Keyspace.lt(Last(node2.pivotTable), rpivot)
-  ensures forall key | key in node2.buckets[0].b :: Keyspace.lte(lpivot, key)
-  ensures forall key | key in Last(node2.buckets).b :: Keyspace.lt(key, rpivot)
   {
-    reveal_CutoffNodeAndKeepLeft();
-    reveal_CutoffNodeAndKeepRight();
-    if (|node2.pivotTable| > 0) {
-      assert node2.pivotTable[0]
-          == node1.pivotTable[|node1.pivotTable| - |node2.pivotTable|];
-      Keyspace.IsStrictlySortedImpliesLte(node1.pivotTable, 0, |node1.pivotTable| - |node2.pivotTable|);
-    }
-    assert |node2.pivotTable| > 0 ==> Keyspace.lt(lpivot, node2.pivotTable[0]);
-    assert |node2.pivotTable| > 0 ==> Keyspace.lt(Last(node2.pivotTable), rpivot);
-    assert forall key | key in node2.buckets[0].b :: Keyspace.lte(lpivot, key);
-    assert forall key | key in Last(node2.buckets).b :: Keyspace.lt(key, rpivot);
+    && BoundedKey(node.pivotTable, lpivot)
+    && (rpivot.Some? ==> ValidLeftCutOffKey(node.pivotTable, rpivot.value))
+    && (rpivot.Some? ==> G.Keyspace.lt(node.pivotTable[0].e, rpivot.value))
+    && (rpivot.Some? ==> G.Keyspace.lt(lpivot, rpivot.value))
+    && (rpivot.None? ==> Last(node.pivotTable) == bpl.Keyspace.Max_Element)
   }
 
-  function {:opaque} CutoffNode(node: Node, lpivot: Option<Key>, rpivot: Option<Key>) : (node' : Node)
+  function {:opaque} CutoffNode(node: Node, lpivot: Key, rpivot: Option<Key>) : (node' : Node)
   requires WFNode(node)
+  requires ValidSplitKey(node, lpivot, rpivot)
   ensures node.children.Some? <==> node'.children.Some?
   ensures WFNode(node')
-  ensures lpivot.Some? && |node'.pivotTable| > 0 ==> Keyspace.lt(lpivot.value, node'.pivotTable[0])
-  ensures rpivot.Some? && |node'.pivotTable| > 0 ==> Keyspace.lt(Last(node'.pivotTable), rpivot.value)
-  ensures lpivot.Some? ==> forall key | key in node'.buckets[0].b :: Keyspace.lte(lpivot.value, key)
-  ensures rpivot.Some? ==> forall key | key in Last(node'.buckets).b :: Keyspace.lt(key, rpivot.value)
+  ensures lpivot == node'.pivotTable[0].e
+  ensures forall key | key in node'.buckets[0].b :: G.Keyspace.lte(lpivot, key)
+  ensures rpivot.Some? ==> Last(node'.pivotTable) == KeyToElement(rpivot.value)
+  ensures rpivot.Some? ==> forall key | key in Last(node'.buckets).b :: G.Keyspace.lt(key, rpivot.value)
   ensures G.Successors(node') <= G.Successors(node)
   ensures WeightBucketList(node'.buckets) <= WeightBucketList(node.buckets)
   ensures |node'.buckets| <= |node.buckets|
   {
-    match lpivot {
+    match rpivot {
       case None => (
-        match rpivot {
-          case None => (
-            node
-          )
-          case Some(rpivot) => (
-            CutoffNodeAndKeepLeft(node, rpivot)
-          )
-        }
+        CutoffNodeAndKeepRight(node, lpivot)
       )
-      case Some(lpivot) => (
-        match rpivot {
-          case None => (
-            CutoffNodeAndKeepRight(node, lpivot)
-          )
-          case Some(rpivot) => (
-            var node1 := CutoffNodeAndKeepLeft(node, rpivot);
-            var node' := CutoffNodeAndKeepRight(node1, lpivot);
-
-            CutoffNodeCorrect(node, node1, node', lpivot, rpivot);
-
-            node'
-          )
-        }
+      case Some(rpivot) => (
+          var node1 := CutoffNodeAndKeepLeft(node, rpivot);
+          var node' := CutoffNodeAndKeepRight(node1, lpivot);
+          CutoffNodeCorrect(node, node1, node', lpivot, rpivot);
+          node'
       )
     }
   }
 
-  //// Split
+  lemma CutoffNodeCorrect(node: Node, node1: Node, node2: Node, lpivot: Key, rpivot: Key)
+  requires WFNode(node)
+  requires ValidLeftCutOffKey(node.pivotTable, rpivot)
+  requires node1 == CutoffNodeAndKeepLeft(node, rpivot);
+  requires BoundedKey(node1.pivotTable, lpivot)
+  requires node2 == CutoffNodeAndKeepRight(node1, lpivot);
+  ensures lpivot == node2.pivotTable[0].e
+  ensures Last(node2.pivotTable) == KeyToElement(rpivot)
+  ensures forall key | key in node2.buckets[0].b :: G.Keyspace.lte(lpivot, key)
+  ensures forall key | key in Last(node2.buckets).b :: G.Keyspace.lt(key, rpivot)
+  {
+    reveal_CutoffNodeAndKeepLeft();
+    reveal_CutoffNodeAndKeepRight();
+  }
 
+  //// Split
   function SplitChildLeft(child: Node, num_children_left: int) : Node
-  requires 0 <= num_children_left - 1 <= |child.pivotTable|
+  requires 0 <= num_children_left - 1 <= |child.pivotTable| - 2
   requires child.children.Some? ==> 0 <= num_children_left <= |child.children.value|
   requires 0 <= num_children_left <= |child.buckets|
   {
     Node(
-      child.pivotTable[ .. num_children_left - 1 ],
+      child.pivotTable[ .. num_children_left + 1],
       if child.children.Some? then Some(child.children.value[ .. num_children_left ]) else None,
       child.buckets[ .. num_children_left ]
     )
   }
 
   function SplitChildRight(child: Node, num_children_left: int) : Node
-  requires 0 <= num_children_left <= |child.pivotTable|
+  requires 0 <= num_children_left <= |child.pivotTable| - 1
   requires child.children.Some? ==> 0 <= num_children_left <= |child.children.value|
   requires 0 <= num_children_left <= |child.buckets|
   {
@@ -547,18 +567,37 @@ module PivotBetreeSpec {
   }
 
   function SplitParent(fused_parent: Node, pivot: Key, slot_idx: int, left_childref: Reference, right_childref: Reference) : Node
-  requires 0 <= slot_idx <= |fused_parent.pivotTable|
+  requires 0 <= slot_idx < NumBuckets(fused_parent.pivotTable)
   requires fused_parent.children.Some?
   requires fused_parent.children.Some? ==> 0 <= slot_idx < |fused_parent.children.value|
   requires 0 <= slot_idx < |fused_parent.buckets|
   {
     Node(
-      insert(fused_parent.pivotTable, pivot, slot_idx),
+      insert(fused_parent.pivotTable, KeyToElement(pivot), slot_idx+1),
       Some(replace1with2(fused_parent.children.value, left_childref, right_childref, slot_idx)),
       SplitBucketInList(fused_parent.buckets, slot_idx, pivot)
     )
   }
 
+  function getlbound(parent: Node, slot: int) : Key
+  requires WFNode(parent)
+  requires parent.children.Some?
+  requires 0 <= slot < |parent.children.value|
+  {
+    GetKey(parent.pivotTable, slot)
+  }
+
+  function getubound(parent: Node, slot: int) : Option<Key>
+  requires WFNode(parent)
+  requires parent.children.Some?
+  requires 0 <= slot < |parent.children.value|
+  {
+    if parent.pivotTable[slot+1].Element? 
+    then Some(GetKey(parent.pivotTable, slot+1)) 
+    else None
+  }
+
+  // a defined set of lock ordering, what counts as smaller, only things that go down the same node has a notion of ordering
   predicate ValidSplit(f: NodeFusion)
   {
     && WFNode(f.fused_parent)
@@ -567,15 +606,22 @@ module PivotBetreeSpec {
     && f.fused_parent.children.Some?
     && 0 <= f.slot_idx < |f.fused_parent.buckets|
     && |f.fused_parent.buckets| <= MaxNumChildren() - 1
+  
+    && var lbound :=  getlbound(f.fused_parent, f.slot_idx);
+    && var ubound :=  getubound(f.fused_parent, f.slot_idx);
 
-    && var lbound := (if f.slot_idx > 0 then Some(f.fused_parent.pivotTable[f.slot_idx - 1]) else None);
-    && var ubound := (if f.slot_idx < |f.fused_parent.pivotTable| then Some(f.fused_parent.pivotTable[f.slot_idx]) else None);
+    && ValidSplitKey(f.fused_child, lbound, ubound)
+    && ValidSplitKey(f.fused_parent, lbound, ubound)
     && var child := CutoffNode(f.fused_child, lbound, ubound);
 
     && 1 <= f.num_children_left < |child.buckets|
     && f.fused_parent.children.value[f.slot_idx] == f.fused_childref
-    && child.pivotTable[f.num_children_left - 1] == f.pivot
-    && Route(f.fused_parent.pivotTable, f.pivot) == f.slot_idx
+
+    && bpl.Keyspace.lte(f.fused_child.pivotTable[0], f.fused_parent.pivotTable[f.slot_idx])
+    && bpl.Keyspace.lte(f.fused_parent.pivotTable[f.slot_idx+1], Last(f.fused_child.pivotTable))
+
+    && child.pivotTable[f.num_children_left].e == f.pivot
+    && PivotInsertable(f.fused_parent.pivotTable,  f.slot_idx+1, f.pivot)
 
     && (f.left_childref == f.right_childref ==> f.left_child == f.right_child)
 
@@ -606,6 +652,9 @@ module PivotBetreeSpec {
 
   //// Merge
 
+  // 0 index children is negative infinity to pivot[0]
+  // f.pivot == the end of the pivot
+
   predicate ValidMerge(f: NodeFusion)
   {
     && WFNode(f.split_parent)
@@ -613,7 +662,7 @@ module PivotBetreeSpec {
     && WFNode(f.right_child)
     && 0 <= f.slot_idx < |f.split_parent.buckets| - 1
     && f.num_children_left == |f.left_child.buckets|
-    && f.split_parent.pivotTable[f.slot_idx] == f.pivot
+    && f.split_parent.pivotTable[f.slot_idx+1].e == f.pivot
     && f.split_parent.children.Some?
     && f.split_parent.children.value[f.slot_idx] == f.left_childref
     && f.split_parent.children.value[f.slot_idx + 1] == f.right_childref
@@ -623,7 +672,7 @@ module PivotBetreeSpec {
     && (f.left_childref == f.right_childref ==> f.left_child == f.right_child)
 
     && f.fused_parent == Node(
-      remove(f.split_parent.pivotTable, f.slot_idx),
+      remove(f.split_parent.pivotTable, f.slot_idx+1),
       Some(replace2with1(f.split_parent.children.value, f.fused_childref, f.slot_idx)),
       MergeBucketsInList(f.split_parent.buckets, f.slot_idx)
     )
@@ -632,15 +681,17 @@ module PivotBetreeSpec {
     // but we currently don't track that as an invariant... should we?
     && (f.left_child.children.Some? ==> f.right_child.children.Some?)
     && (f.left_child.children.None? ==> f.right_child.children.None?)
+  
+    && var lbound :=  getlbound(f.split_parent, f.slot_idx);
+    && var ubound :=  getubound(f.split_parent, f.slot_idx);
 
-    && var lbound := (if f.slot_idx > 0 then Some(f.split_parent.pivotTable[f.slot_idx - 1]) else None);
-    && var ubound := (if f.slot_idx + 1 < |f.split_parent.pivotTable| then Some(f.split_parent.pivotTable[f.slot_idx + 1]) else None);
-
+    && ValidSplitKey(f.left_child, lbound, Some(f.pivot))
+    && ValidSplitKey(f.right_child, f.pivot, ubound)
     && var left := CutoffNode(f.left_child, lbound, Some(f.pivot));
-    && var right := CutoffNode(f.right_child, Some(f.pivot), ubound);
+    && var right := CutoffNode(f.right_child, f.pivot, ubound);
 
     && f.fused_child == Node(
-      concat3(left.pivotTable, f.pivot, right.pivotTable),
+      concat3(left.pivotTable[..|left.pivotTable|-1], KeyToElement(f.pivot), right.pivotTable[1..]),
       if left.children.Some? then Some(left.children.value + right.children.value) else None,
       left.buckets + right.buckets
     )
@@ -667,14 +718,15 @@ module PivotBetreeSpec {
 
   //// Repivot
 
-  datatype Repivot = Repivot(ref: Reference, leaf: Node, pivots: seq<Key>)
+  datatype Repivot = Repivot(ref: Reference, leaf: Node, pivots: PivotTable)
 
   predicate ValidRepivot(r: Repivot)
   {
     && WFNode(r.leaf)
+    && |r.pivots| <= MaxNumChildren() + 1
+    && BoundedBucketList(r.leaf.buckets, r.leaf.pivotTable)
+    && ContainsAllKeys(r.pivots) 
     && r.leaf.children.None?
-    && WFPivots(r.pivots)
-    && |r.pivots| <= MaxNumChildren() - 1
   }
 
   function RepivotReads(r: Repivot) : seq<ReadOp>
@@ -685,19 +737,31 @@ module PivotBetreeSpec {
     ]
   }
 
-  function ApplyRepivot(leaf: Node, pivots: seq<Key>) : (leaf': Node)
-  requires WFNode(leaf)
-  requires leaf.children.None?
-  requires WFPivots(pivots)
+  lemma PivotsHasAllKeys(pt: PivotTable)
+  requires ContainsAllKeys(pt)
+  ensures (forall key : Key | MS.InDomain(key) :: BoundedKey(pt, key))
   {
-    Node(pivots, None, SplitBucketOnPivots(JoinBucketList(leaf.buckets), pivots))
+    forall key : Key | MS.InDomain(key)
+    ensures BoundedKey(pt, key)
+    {
+      G.Keyspace.SeqComparison.reveal_lte();
+    }
+  }
+
+  function ApplyRepivot(r: Repivot) : (leaf': Node)
+  requires ValidRepivot(r)
+  {
+    PivotsHasAllKeys(r.pivots);
+    BoundedBucketListJoin(r.leaf.buckets, r.pivots);
+    var leaf' := Node(r.pivots, None, SplitBucketOnPivots(JoinBucketList(r.leaf.buckets), r.pivots));
+    leaf'
   }
 
   function RepivotOps(r: Repivot) : seq<Op>
   requires ValidRepivot(r)
   {
     [
-      G.WriteOp(r.ref, ApplyRepivot(r.leaf, r.pivots))
+      G.WriteOp(r.ref, ApplyRepivot(r))
     ]
   }
 
@@ -769,4 +833,5 @@ module PivotBetreeSpec {
       case BetreeRepivot(r) => uiop.NoOp?
     }
   }
+
 }
